Solve Equiv.v!

plf/Equiv.v
@@ -186,7 +186,17 @@ Theorem skip_right : forall c,
     <{ c ; skip }>
     c.
 Proof.
-  (* FILL IN HERE *) Admitted.
+  intros c st st'.
+  split; intros H.
+  - (* -> *)
+    inversion H. subst.
+    inversion H5. subst.
+    assumption.
+  - (* <- *)
+    apply E_Seq with st'.
+    + assumption.
+    + apply E_Skip.
+Qed.
 (** [] *)
 
 (** Similarly, here is a simple equivalence that optimizes [if]
@@ -278,7 +288,20 @@ Theorem if_false : forall b c1 c2,
     <{ if b then c1 else c2 end }>
     c2.
 Proof.
-  (* FILL IN HERE *) Admitted.
+  intros b c1 c2 Hb.
+  split; intros H.
+  - (* -> *)
+    inversion H; subst.
+    + (* b evaluates to false *)
+      unfold bequiv in Hb. simpl in Hb.
+      rewrite Hb in H5.
+      discriminate.
+    + (* b evaluates to true *)
+      assumption.
+  - (* <- *)
+    apply E_IfFalse; try assumption.
+    unfold bequiv in Hb. auto.
+Qed.
 (** [] *)
 
 (** **** Exercise: 3 stars, standard (swap_if_branches)
@@ -291,7 +314,21 @@ Theorem swap_if_branches : forall b c1 c2,
     <{ if b then c1 else c2 end }>
     <{ if ~ b then c2 else c1 end }>.
 Proof.
-  (* FILL IN HERE *) Admitted.
+  intros b c1 c2.
+  split; intros; inversion H; subst.
+  - apply E_IfFalse.
+    * simpl. rewrite H5. reflexivity.
+    * assumption.
+  - apply E_IfTrue.
+    * simpl. rewrite H5. reflexivity.
+    * assumption.
+  - apply E_IfFalse.
+    * simpl in H5. destruct (beval st b); [discriminate | reflexivity].
+    * assumption.
+  - apply E_IfTrue.
+    * simpl in H5. destruct (beval st b); [reflexivity | discriminate].
+    * assumption.
+Qed.
 (** [] *)
 
 (** For [while] loops, we can give a similar pair of theorems.  A loop
@@ -394,7 +431,10 @@ Theorem while_true : forall b c,
     <{ while b do c end }>
     <{ while true do skip end }>.
 Proof.
-  (* FILL IN HERE *) Admitted.
+  intros b c Hb st st'.
+  split; intros H; apply while_true_nonterm in H; intuition.
+  unfold bequiv. reflexivity.
+Qed.
 (** [] *)
 
 (** A more interesting fact about [while] commands is that any number
@@ -438,7 +478,17 @@ Proof.
 Theorem seq_assoc : forall c1 c2 c3,
   cequiv <{(c1;c2);c3}> <{c1;(c2;c3)}>.
 Proof.
-  (* FILL IN HERE *) Admitted.
+  intros c1 c2 c3 st st'.
+  split; intros H; inversion H; subst.
+  - inversion H2; subst.
+    apply E_Seq with (st':=st'1).
+    + assumption.
+    + apply E_Seq with (st':=st'0); assumption.
+  - inversion H5; subst.
+    apply E_Seq with (st':=st'1).
+    + apply E_Seq with (st':=st'0); assumption.
+    + assumption.
+Qed.
 (** [] *)
 
 (** Proving program properties involving assignments is one place
@@ -467,7 +517,14 @@ Theorem assign_aequiv : forall (X : string) (a : aexp),
   aequiv <{ X }> a ->
   cequiv <{ skip }> <{ X := a }>.
 Proof.
-  (* FILL IN HERE *) Admitted.
+  intros X a Ha.
+  unfold aequiv in Ha.
+  split; intro H; inversion H; subst; clear H.
+  - assert (H : st' =[ X := a ]=> (X !-> st' X ; st')).
+    { constructor. rewrite <- Ha. reflexivity. }
+    rewrite t_update_same in H. assumption.
+  - rewrite <- (Ha st). rewrite t_update_same. constructor.
+Qed.
 (** [] *)
 
 (** **** Exercise: 2 stars, standard (equiv_classes) *)
@@ -532,7 +589,7 @@ Definition prog_i : com :=
      end }>.
 
 Definition equiv_classes : list (list com)
-  (* REPLACE THIS LINE WITH ":= _your_definition_ ." *). Admitted.
+  := [[prog_a; prog_d]; [prog_b; prog_e]; [prog_c; prog_h]; [prog_f; prog_g];  [prog_i]].
 
 (* Do not modify the following line: *)
 Definition manual_grade_for_equiv_classes : option (nat*string) := None.
@@ -725,7 +782,10 @@ Theorem CSeq_congruence : forall c1 c1' c2 c2',
   cequiv c1 c1' -> cequiv c2 c2' ->
   cequiv <{ c1;c2 }> <{ c1';c2' }>.
 Proof.
-  (* FILL IN HERE *) Admitted.
+  intros c1 c1' c2 c2' Hce1 Hce2.
+  split; intros H; inversion H; subst; clear H;
+    (apply E_Seq with (st':=st'0); [apply Hce1 | apply Hce2]; assumption).
+Qed.
 (** [] *)
 
 (** **** Exercise: 3 stars, standard (CIf_congruence) *)
@@ -734,7 +794,21 @@ Theorem CIf_congruence : forall b b' c1 c1' c2 c2',
   cequiv <{ if b then c1 else c2 end }>
          <{ if b' then c1' else c2' end }>.
 Proof.
-  (* FILL IN HERE *) Admitted.
+  intros b b' c1 c1' c2 c2' Hbe Hce1 Hce2.
+  split; intros H; inversion H; subst; clear H.
+  - apply E_IfTrue.
+    + rewrite <- Hbe. assumption.
+    + apply Hce1. assumption.
+  - apply E_IfFalse.
+    + rewrite <- Hbe. assumption.
+    + apply Hce2. assumption.
+  - apply E_IfTrue.
+    + rewrite -> Hbe. assumption.
+    + apply Hce1. assumption.
+  - apply E_IfFalse.
+    + rewrite -> Hbe. assumption.
+    + apply Hce2. assumption.
+Qed.
 (** [] *)
 
 (** For example, here are two equivalent programs and a proof of their
@@ -1115,9 +1189,25 @@ Proof.
        become constants after folding *)
       simpl. destruct (n =? n0); reflexivity.
   - (* BLe *)
-    (* FILL IN HERE *) admit.
+    simpl.
+    remember (fold_constants_aexp a1) as a1' eqn:Heqa1'.
+    remember (fold_constants_aexp a2) as a2' eqn:Heqa2'.
+    replace (aeval st a1) with (aeval st a1') by
+       (subst a1'; rewrite <- fold_constants_aexp_sound; reflexivity).
+    replace (aeval st a2) with (aeval st a2') by
+       (subst a2'; rewrite <- fold_constants_aexp_sound; reflexivity).
+    destruct a1'; destruct a2'; try reflexivity.
+    simpl. destruct (n <=? n0); reflexivity.
   - (* BGt *)
-    (* FILL IN HERE *) admit.
+    simpl.
+    remember (fold_constants_aexp a1) as a1' eqn:Heqa1'.
+    remember (fold_constants_aexp a2) as a2' eqn:Heqa2'.
+    replace (aeval st a1) with (aeval st a1') by
+       (subst a1'; rewrite <- fold_constants_aexp_sound; reflexivity).
+    replace (aeval st a2) with (aeval st a2') by
+       (subst a2'; rewrite <- fold_constants_aexp_sound; reflexivity).
+    destruct a1'; destruct a2'; try reflexivity.
+    simpl. destruct (n <=? n0); reflexivity.
   - (* BNot *)
     simpl. remember (fold_constants_bexp b) as b' eqn:Heqb'.
     rewrite IHb.
@@ -1128,7 +1218,7 @@ Proof.
     remember (fold_constants_bexp b2) as b2' eqn:Heqb2'.
     rewrite IHb1. rewrite IHb2.
     destruct b1'; destruct b2'; reflexivity.
-(* FILL IN HERE *) Admitted.
+Qed.
 (** [] *)
 
 (** **** Exercise: 3 stars, standard (fold_constants_com_sound)
@@ -1159,7 +1249,13 @@ Proof.
       apply trans_cequiv with c2; try assumption.
       apply if_false; assumption.
   - (* while *)
-    (* FILL IN HERE *) Admitted.
+    assert (bequiv b (fold_constants_bexp b)). {
+      apply fold_constants_bexp_sound. }
+    destruct (fold_constants_bexp b) eqn:Heqb;
+      try (apply CWhile_congruence; assumption).
+    + apply while_true. assumption.
+    + apply while_false. assumption.
+Qed.
 (** [] *)
 
 (* ================================================================= *)
@@ -1196,20 +1292,47 @@ Proof.
 *)
 
 Fixpoint optimize_0plus_aexp (a : aexp) : aexp
-  (* REPLACE THIS LINE WITH ":= _your_definition_ ." *). Admitted.
+  := match a with
+  | ANum n       => ANum n
+  | AId x        => AId x
+  | <{ a1 + a2 }>  =>
+    match (optimize_0plus_aexp a1,
+           optimize_0plus_aexp a2)
+    with
+    | (ANum 0, a2') => a2'
+    | (a1', a2') => <{ a1' + a2' }>
+    end
+  | <{ a1 - a2 }> => <{ optimize_0plus_aexp a1 - optimize_0plus_aexp a2 }>
+  | <{ a1 * a2 }> => <{ optimize_0plus_aexp a1 * optimize_0plus_aexp a2 }>
+  end.
 
 Fixpoint optimize_0plus_bexp (b : bexp) : bexp
-  (* REPLACE THIS LINE WITH ":= _your_definition_ ." *). Admitted.
+  := match b with
+  | <{true}>       => <{true}>
+  | <{false}>      => <{false}>
+  | <{ a1 = a2 }>  => <{ optimize_0plus_aexp a1 = optimize_0plus_aexp a2 }>
+  | <{ a1 <> a2 }>  => <{ optimize_0plus_aexp a1 <> optimize_0plus_aexp a2 }>
+  | <{ a1 <= a2 }>  => <{ optimize_0plus_aexp a1 <= optimize_0plus_aexp a2 }>
+  | <{ a1 > a2 }>  => <{ optimize_0plus_aexp a1 > optimize_0plus_aexp a2 }>
+  | <{ ~ b1 }>     => <{ ~ optimize_0plus_bexp b1 }>
+  | <{ b1 && b2 }> => <{ optimize_0plus_bexp b1 && optimize_0plus_bexp b2 }>
+  end.
 
 Fixpoint optimize_0plus_com (c : com) : com
-  (* REPLACE THIS LINE WITH ":= _your_definition_ ." *). Admitted.
+  := match c with
+  | <{ skip }> => <{ skip }>
+  | <{ x := a }> => <{ x := optimize_0plus_aexp a }>
+  | <{ c1 ; c2 }>  => <{ optimize_0plus_com c1 ; optimize_0plus_com c2 }>
+  | <{ if b then c1 else c2 end }> => <{ if optimize_0plus_bexp b then optimize_0plus_com c1 else optimize_0plus_com c2 end }>
+  | <{ while b do c1 end }> => <{ while optimize_0plus_bexp b do optimize_0plus_com c1 end }>
+  end.
 
 Example test_optimize_0plus:
     optimize_0plus_com
        <{ while X <> 0 do X := 0 + X - 1 end }>
   =    <{ while X <> 0 do X := X - 1 end }>.
 Proof.
-  (* FILL IN HERE *) Admitted.
+  reflexivity. Qed.
 
 (** Prove that these three functions are sound, as we did for
     [fold_constants_*].  Make sure you use the congruence lemmas in the
@@ -1218,17 +1341,45 @@ Proof.
 Theorem optimize_0plus_aexp_sound:
   atrans_sound optimize_0plus_aexp.
 Proof.
-  (* FILL IN HERE *) Admitted.
+  unfold atrans_sound. intros a. unfold aequiv. intros st.
+  induction a; simpl;
+    try reflexivity;
+    try (destruct (optimize_0plus_aexp a1); destruct (optimize_0plus_aexp a2));
+    try (rewrite IHa1; rewrite IHa2; try (destruct n); reflexivity).
+Qed.
 
 Theorem optimize_0plus_bexp_sound :
   btrans_sound optimize_0plus_bexp.
 Proof.
-  (* FILL IN HERE *) Admitted.
+  unfold btrans_sound. intros b. unfold bequiv. intros st.
+  induction b; simpl;
+    try reflexivity;
+    try (rewrite <- (optimize_0plus_aexp_sound a1); rewrite <- (optimize_0plus_aexp_sound a2); reflexivity).
+  - (* BNot *)
+    rewrite IHb. reflexivity.
+  - (* BAnd *)
+    rewrite IHb1. rewrite IHb2. reflexivity.
+Qed.
 
 Theorem optimize_0plus_com_sound :
   ctrans_sound optimize_0plus_com.
 Proof.
-  (* FILL IN HERE *) Admitted.
+  unfold ctrans_sound. intros c.
+  induction c; simpl.
+  - (* skip *) apply refl_cequiv.
+  - (* := *)
+    apply CAsgn_congruence.
+    apply optimize_0plus_aexp_sound.
+  - (* ; *) apply CSeq_congruence; assumption.
+  - apply CIf_congruence.
+    + apply optimize_0plus_bexp_sound.
+    + assumption.
+    + assumption.
+  - (* while *)
+    apply CWhile_congruence.
+    + apply optimize_0plus_bexp_sound.
+    + assumption.
+Qed.
 
 (** Finally, let's define a compound optimizer on commands that first
     folds constants (using [fold_constants_com]) and then eliminates
@@ -1241,7 +1392,12 @@ Definition optimizer (c : com) := optimize_0plus_com (fold_constants_com c).
 Theorem optimizer_sound :
   ctrans_sound optimizer.
 Proof.
-  (* FILL IN HERE *) Admitted.
+  unfold ctrans_sound. unfold optimizer. intros c. remember c as c'.
+  induction c;
+    apply trans_cequiv with (c2 := fold_constants_com c');
+    try (apply fold_constants_com_sound);
+    try (apply optimize_0plus_com_sound).
+Qed.
 (** [] *)
 
 (* ################################################################# *)
@@ -1388,14 +1544,53 @@ Lemma aeval_weakening : forall x st a ni,
   var_not_used_in_aexp x a ->
   aeval (x !-> ni ; st) a = aeval st a.
 Proof.
-  (* FILL IN HERE *) Admitted.
+  intros.
+  induction H; simpl.
+  - reflexivity.
+  - apply t_update_neq. assumption.
+  - rewrite IHvar_not_used_in_aexp1. rewrite IHvar_not_used_in_aexp2. reflexivity.
+  - rewrite IHvar_not_used_in_aexp1. rewrite IHvar_not_used_in_aexp2. reflexivity.
+  - rewrite IHvar_not_used_in_aexp1. rewrite IHvar_not_used_in_aexp2. reflexivity.
+Qed.
 
 (** Using [var_not_used_in_aexp], formalize and prove a correct version
     of [subst_equiv_property]. *)
 
-(* FILL IN HERE
-
-    [] *)
+Theorem better_subst_equiv : forall x1 x2 a1 a2,
+    var_not_used_in_aexp x1 a1 ->
+    cequiv <{ x1 := a1; x2 := a2 }>
+    <{ x1 := a1; x2 := subst_aexp x1 a1 a2 }>.
+Proof.
+  intros.
+  unfold cequiv. intros.
+  split; intros Hceval; inversion Hceval; inversion H5; inversion H2; subst; clear H2 H5 Hceval.
+  - apply E_Seq with (st' := (x1 !-> aeval st a1; st)).
+    + apply E_Asgn. reflexivity.
+    + apply E_Asgn.
+      induction a2.
+      * (* ANum *) reflexivity.
+      * (* AId *) unfold subst_aexp. destruct (x1 =? x)%string eqn:E.
+        ** assert (x1 = x). { apply String.eqb_eq. apply E. }.
+            rewrite <- H0. simpl. rewrite t_update_eq.
+            apply aeval_weakening. assumption.
+        ** reflexivity.
+      * (* APlus *) simpl. rewrite IHa2_1. rewrite IHa2_2. reflexivity.
+      * (* AMinus *) simpl. rewrite IHa2_1. rewrite IHa2_2. reflexivity.
+      * (* AMult *) simpl. rewrite IHa2_1. rewrite IHa2_2. reflexivity.
+  - apply E_Seq with (st' := (x1 !-> aeval st a1; st)).
+    + apply E_Asgn. reflexivity.
+    + apply E_Asgn.
+      induction a2.
+      * (* ANum *) reflexivity.
+      * (* AId *) unfold subst_aexp. destruct (x1 =? x)%string eqn:E.
+        ** assert (x1 = x). { apply String.eqb_eq. apply E. }.
+            rewrite <- H0. simpl. rewrite t_update_eq.
+            symmetry. apply aeval_weakening. assumption.
+        ** reflexivity.
+      * (* APlus *) simpl. rewrite IHa2_1. rewrite IHa2_2. reflexivity.
+      * (* AMinus *) simpl. rewrite IHa2_1. rewrite IHa2_2. reflexivity.
+      * (* AMult *) simpl. rewrite IHa2_1. rewrite IHa2_2. reflexivity.
+Qed.
 
 (** **** Exercise: 3 stars, standard (inequiv_exercise)
 
@@ -1404,7 +1599,16 @@ Proof.
 Theorem inequiv_exercise:
   ~ cequiv <{ while true do skip end }> <{ skip }>.
 Proof.
-  (* FILL IN HERE *) Admitted.
+  unfold cequiv. intros contra.
+  assert (H1: forall st st', ~( st =[ while true do skip end ]=> st' )).
+    { intros. apply while_true_nonterm. apply refl_bequiv. }
+  assert (H2: exists st st', st =[ skip ]=> st').
+    { exists empty_st. exists empty_st. apply E_Skip. }
+  destruct H2 as [st [st' H2]].
+  apply (H1 st st').
+  apply contra.
+  assumption.
+Qed.
 (** [] *)
 
 (* ################################################################# *)
@@ -1521,7 +1725,8 @@ Inductive ceval : com -> state -> state -> Prop :=
       st  =[ c ]=> st' ->
       st' =[ while b do c end ]=> st'' ->
       st  =[ while b do c end ]=> st''
-(* FILL IN HERE *)
+  | E_Havoc : forall st n x,
+      st  =[ havoc x ]=> (x !-> n ; st)
 
   where "st =[ c ]=> st'" := (ceval c st st').
 
@@ -1530,12 +1735,15 @@ Inductive ceval : com -> state -> state -> Prop :=
 
 Example havoc_example1 : empty_st =[ havoc X ]=> (X !-> 0).
 Proof.
-(* FILL IN HERE *) Admitted.
+  apply E_Havoc. Qed.
 
 Example havoc_example2 :
   empty_st =[ skip; havoc Z ]=> (Z !-> 42).
 Proof.
-(* FILL IN HERE *) Admitted.
+  apply E_Seq with (st' := empty_st).
+  + apply E_Skip.
+  + apply E_Havoc.
+Qed.
 
 (* Do not modify the following line: *)
 Definition manual_grade_for_Check_rule_for_HAVOC : option (nat*string) := None.
@@ -1568,7 +1776,25 @@ Proof.
   (* Hint: You may want to use [t_update_permute] at some point,
      in which case you'll probably be left with [X <> Y] as a
      hypothesis. You can use [discriminate] to discharge this. *)
-  (* FILL IN HERE *) Admitted.
+  left.
+  unfold cequiv. unfold pXY. unfold pYX. split; intros Hceval.
+  - inversion Hceval. inversion H1. inversion H4. subst.
+    assert (H: st =[ havoc Y; havoc X ]=> (X !-> n; Y !-> n0; st)).
+    { apply E_Seq with (st' := (Y !-> n0; st)).
+      + apply E_Havoc.
+      + apply E_Havoc. }
+    assert (E: (Y !-> n0; X !-> n; st) = (X !-> n; Y !-> n0; st)).
+    { apply t_update_permute. discriminate. }
+    rewrite E. assumption.
+  - inversion Hceval. inversion H1. inversion H4. subst.
+    assert (H: st =[ havoc X; havoc Y ]=> (Y !-> n; X !-> n0; st)).
+    { apply E_Seq with (st' := (X !-> n0; st)).
+      + apply E_Havoc.
+      + apply E_Havoc. }
+    assert (E: (X !-> n0; Y !-> n; st) = (Y !-> n; X !-> n0;  st)).
+    { apply t_update_permute. discriminate. }
+    rewrite E. assumption.
+Qed.
 (** [] *)
 
 (** **** Exercise: 4 stars, standard, optional (havoc_copy)
@@ -1587,7 +1813,24 @@ Definition pcopy :=
 
 Theorem ptwice_cequiv_pcopy :
   cequiv ptwice pcopy \/ ~cequiv ptwice pcopy.
-Proof. (* FILL IN HERE *) Admitted.
+Proof.
+  right.
+  unfold cequiv. intros contra.
+  assert (H: empty_st =[ ptwice ]=> (Y !-> 42; X !-> 43)).
+  { apply E_Seq with (st' := (X !-> 43)); apply E_Havoc. }
+  apply contra in H.
+  inversion H. inversion H2. inversion H5. subst.
+  simpl in H13. rewrite t_update_eq in H13.
+  apply equal_f with (x := Y) in H13 as E1.
+  repeat rewrite t_update_eq in E1.
+  apply equal_f with (x := X) in H13 as E2.
+  assert (Hp: forall m n, (Y !-> m; X !-> n) = (X !-> n; Y !-> m)).
+  { intros. apply t_update_permute. discriminate. }
+  repeat rewrite Hp in E2. clear Hp.
+  repeat rewrite t_update_eq in E2.
+  rewrite E1 in E2.
+  discriminate E2.
+Qed.
 (** [] *)
 
 (** The definition of program equivalence we are using here has some
@@ -1623,12 +1866,33 @@ Definition p2 : com :=
 
 Lemma p1_may_diverge : forall st st', st X <> 0 ->
   ~ st =[ p1 ]=> st'.
-Proof. (* FILL IN HERE *) Admitted.
+Proof.
+  intros. unfold not. unfold p1. intros contra.
+  remember <{ while ~ X = 0 do havoc Y; X := X + 1 end }> as p eqn:Heqp.
+  induction contra; try discriminate; inversion Heqp; subst.
+  - apply negb_false_iff in H0.
+    apply eqb_eq in H0.
+    contradiction.
+  - apply IHcontra2.
+    + inversion contra1. inversion H6. subst.
+      simpl. rewrite t_update_eq. lia.
+    + reflexivity.
+Qed.
 
 Lemma p2_may_diverge : forall st st', st X <> 0 ->
   ~ st =[ p2 ]=> st'.
 Proof.
-(* FILL IN HERE *) Admitted.
+  intros.
+  unfold not. unfold p2. intros contra.
+  remember <{ while ~ X = 0 do skip end }> as p eqn:Heqp.
+  induction contra; try discriminate; inversion Heqp; subst.
+  - apply negb_false_iff in H0.
+    apply eqb_eq in H0.
+    contradiction.
+  -  apply IHcontra2.
+    + inversion contra1. subst. assumption.
+    + reflexivity.
+Qed.
 (** [] *)
 
 (** **** Exercise: 4 stars, advanced (p1_p2_equiv)
@@ -1637,7 +1901,20 @@ Proof.
     equivalent. *)
 
 Theorem p1_p2_equiv : cequiv p1 p2.
-Proof. (* FILL IN HERE *) Admitted.
+Proof.
+  unfold cequiv. intros.
+  split; intros; inversion H; try discriminate; subst; try (apply E_WhileFalse; assumption).
+  - exfalso.
+    apply (p1_may_diverge st st').
+    + simpl in H2. apply negb_true_iff in H2.
+      destruct (st X); discriminate; lia.
+    + assumption.
+  - exfalso.
+    apply (p2_may_diverge st st').
+    + simpl in H2. apply negb_true_iff in H2.
+      destruct (st X); discriminate; lia.
+    + assumption.
+Qed.
 (** [] *)
 
 (** **** Exercise: 4 stars, advanced (p3_p4_inequiv)
@@ -1658,7 +1935,34 @@ Definition p4 : com :=
      Z := 1 }>.
 
 Theorem p3_p4_inequiv : ~ cequiv p3 p4.
-Proof. (* FILL IN HERE *) Admitted.
+Proof.
+  unfold cequiv. unfold not. intros contra.
+  remember (X !-> 1) as st.
+  remember (Z !-> 2; X !-> 0; Z !-> 1; st) as st1.
+  remember (Z !-> 1; X !-> 0; st) as st2.
+  assert (Hp3: st =[ p3 ]=> st1).
+  { apply E_Seq with (st' := (Z !-> 1; st)).
+    - apply E_Asgn. reflexivity.
+    - apply E_WhileTrue with (st' := st1).
+      + simpl. apply negb_true_iff.
+        rewrite Heqst. reflexivity.
+      + apply E_Seq with (st' := (X !-> 0; Z !-> 1; st)).
+        * apply E_Havoc.
+        * rewrite Heqst1. apply E_Havoc.
+      + apply E_WhileFalse.
+        simpl. apply negb_false_iff.
+        rewrite Heqst1. reflexivity. }
+  assert (Hp4: st =[ p4 ]=> st2).
+  { apply E_Seq with (st' := (X !-> 0; st)).
+    - apply E_Asgn. reflexivity.
+    - rewrite Heqst2. apply E_Asgn. reflexivity. }
+  assert (contra1: st =[ p4 ]=> st1).
+  { apply contra. assumption. }
+  inversion Hp3. inversion contra1. inversion H10. subst.
+  simpl in H14. apply equal_f with (x := Z) in H14.
+  repeat rewrite t_update_eq in H14.
+  discriminate.
+Qed.
 (** [] *)
 
 (** **** Exercise: 5 stars, advanced, optional (p5_p6_equiv)
@@ -1680,7 +1984,41 @@ Definition p6 : com :=
   <{ X := 1 }>.
 
 Theorem p5_p6_equiv : cequiv p5 p6.
-Proof. (* FILL IN HERE *) Admitted.
+Proof.
+  unfold cequiv. intros.
+  unfold p5. unfold p6.
+  split; intros Hceval.
+  - remember <{ while X <> 1 do havoc X end }> as p5.
+    induction Hceval; try discriminate; inversion Heqp5; subst.
+    + simpl in H. apply negb_false_iff in H. apply eqb_eq in H.
+      rewrite <- t_update_same with (x := X).
+      rewrite H.
+      apply E_Asgn. reflexivity.
+    + inversion Hceval1. inversion Hceval2; subst.
+      * simpl in H7. apply negb_false_iff in H7. rewrite t_update_eq in H7. apply eqb_eq in H7.
+        apply E_Asgn. simpl. symmetry. assumption.
+      * assert ((X !-> n; st) =[ X := 1 ]=> st'').
+        { apply IHHceval2. reflexivity. }
+        inversion H0; subst.
+        simpl.
+        rewrite t_update_shadow.
+        apply E_Asgn. reflexivity.
+  - remember <{ X := 1 }> as p6.
+    induction Hceval; subst; try discriminate.
+    inversion Heqp6; subst.
+    destruct (eqb_spec (st X) 1) as [E | E].
+    + simpl. replace (X !-> 1; st) with (X !-> st X; st) by (rewrite E; reflexivity).
+      rewrite t_update_same. apply E_WhileFalse.
+      apply negb_false_iff.
+      apply eqb_eq.
+      assumption.
+    + apply E_WhileTrue with (st' := (X !-> 1; st)).
+      * apply negb_true_iff.
+        apply eqb_neq.
+        assumption.
+      * apply E_Havoc.
+      * apply E_WhileFalse. reflexivity.
+Qed.
 (** [] *)
 
 End Himp.
@@ -1701,7 +2039,22 @@ Theorem swap_noninterfering_assignments: forall l1 l2 a1 a2,
     <{ l1 := a1; l2 := a2 }>
     <{ l2 := a2; l1 := a1 }>.
 Proof.
-(* FILL IN HERE *) Admitted.
+  intros l1 l2 a1 a2 H H12 H21.
+  unfold cequiv.
+  split; intros Hceval.
+  - inversion Hceval; inversion H2; inversion H5; subst.
+    rewrite aeval_weakening by (apply H12).
+    rewrite t_update_permute by (apply H).
+    apply E_Seq with (st' := (l2 !-> aeval st a2; st)).
+    + apply E_Asgn. reflexivity.
+    + apply E_Asgn. rewrite aeval_weakening by (apply H21). reflexivity.
+  - inversion Hceval; inversion H2; inversion H5; subst.
+    rewrite aeval_weakening by (apply H21).
+    rewrite t_update_permute by (apply (not_eq_sym H)).
+    apply E_Seq with (st' := (l1 !-> aeval st a1; st)).
+    + apply E_Asgn. reflexivity.
+    + apply E_Asgn. rewrite aeval_weakening by (apply H12). reflexivity.
+Qed.
 (** [] *)
 
 (** **** Exercise: 4 stars, standard, optional (for_while_equiv)
@@ -1753,30 +2106,65 @@ Definition capprox (c1 c2 : com) : Prop := forall (st st' : state),
     the other. *)
 
 Definition c3 : com
-  (* REPLACE THIS LINE WITH ":= _your_definition_ ." *). Admitted.
+  := <{ X := 1 }>.
 Definition c4 : com
-  (* REPLACE THIS LINE WITH ":= _your_definition_ ." *). Admitted.
+  := <{ X := 2 }>.
 
 Theorem c3_c4_different : ~ capprox c3 c4 /\ ~ capprox c4 c3.
-Proof. (* FILL IN HERE *) Admitted.
+Proof.
+  unfold capprox.
+  split; intros contra.
+  - assert (contra1: empty_st =[ c4 ]=> (X !-> 2)).
+    { apply E_Asgn. reflexivity. }
+    assert (contra2: empty_st =[ c4 ]=> (X !-> 1)).
+    { apply contra. apply E_Asgn. reflexivity. }
+    inversion contra1.
+    inversion contra2.
+    subst.
+    clear H3. simpl in H8.
+    apply equal_f with (x := X) in H8.
+    discriminate.
+  - assert (contra1: empty_st =[ c3 ]=> (X !-> 1)).
+    { apply E_Asgn. reflexivity. }
+    assert (contra2: empty_st =[ c3 ]=> (X !-> 2)).
+    { apply contra. apply E_Asgn. reflexivity. }
+    inversion contra1.
+    inversion contra2.
+    subst.
+    clear H3. simpl in H8.
+    apply equal_f with (x := X) in H8.
+    discriminate.
+Qed.
 
 (** Find a program [cmin] that approximates every other program. *)
 
 Definition cmin : com
-  (* REPLACE THIS LINE WITH ":= _your_definition_ ." *). Admitted.
+  := <{ while true do skip end }>.
 
 Theorem cmin_minimal : forall c, capprox cmin c.
-Proof. (* FILL IN HERE *) Admitted.
+Proof.
+  unfold capprox. intros.
+  assert (contra: ~( st =[ cmin ]=> st' )).
+  { apply while_true_nonterm. apply refl_bequiv. }
+  contradiction.
+Qed.
 
 (** Finally, find a non-trivial property which is preserved by
     program approximation (when going from left to right). *)
 
 Definition zprop (c : com) : Prop
-  (* REPLACE THIS LINE WITH ":= _your_definition_ ." *). Admitted.
+  := forall st, exists st', st =[ c ]=> st'.
 
 Theorem zprop_preserving : forall c c',
   zprop c -> capprox c c' -> zprop c'.
-Proof. (* FILL IN HERE *) Admitted.
+Proof.
+  unfold zprop.
+  unfold capprox.
+  intros c c' Hz Hc.
+  intros.
+  destruct (Hz st) as [st' H].
+  exists st'. apply Hc. assumption.
+Qed.
 (** [] *)
 
 (* 2024-01-02 21:54 *)
